end to end proof for first RISCV program

examples/riscv64_test.v
@@ -1,30 +1,66 @@
 Require Import isla.riscv64.riscv64.
 From isla.instructions.riscv64_test Require Import instrs.
 
-Lemma test `{!islaG Σ} `{!threadG} :
+Definition misa_bits : bv 64 :=
+  [BV{64}0x800000000015312d].
+
+Definition riscv_test_spec (x11 : bv 64) : spec :=
+  (sif (bv_unsigned x11 = 1)
+               (scons (SInstrTrap [BV{64} 0x0000000010300010]) snil)
+               (scons (SInstrTrap [BV{64} 0x000000001030000c]) snil)).
+
+Lemma riscv_test `{!islaG Σ} `{!threadG} (x11 : bv 64):
   instr 0x0000000010300000 (Some a0) -∗
   instr 0x0000000010300004 (Some a4) -∗
   instr 0x0000000010300008 (Some a8) -∗
   instr 0x000000001030000c None -∗
   instr 0x0000000010300010 None -∗
   instr_body 0x0000000010300000 (
-    ∃ x11 : bv 64,
     "x10" ↦ᵣ: λ _,
     "x11" ↦ᵣ RVal_Bits x11 ∗
-    "misa" # "bits" ↦ᵣ RVal_Bits (bv_0 64) ∗
-    spec_trace (sif (bv_unsigned x11 = 1)
-               (scons (SInstrTrap [BV{64} 0x0000000010300010]) snil)
-               (scons (SInstrTrap [BV{64} 0x000000001030000c]) snil)) ∗
+    "misa" ↦ᵣ RegVal_Struct [("bits", RVal_Bits misa_bits)] ∗
+    spec_trace (riscv_test_spec x11) ∗
     True
   ).
 Proof.
   iStartProof.
   Time repeat liAStep; liShow.
-  admit.
   Unshelve. all: prepare_sidecond.
-  - admit.
-  - rewrite sif_false //. rename select (_ ≠ x11) into Hx11. contradict Hx11. bv_solve.
-  - admit.
-  - rewrite sif_true //.
-  - admit.
-Admitted.
+  - rewrite /riscv_test_spec sif_false //. rename select (_ ≠ x11) into Hx11. contradict Hx11. bv_solve.
+  - rewrite /riscv_test_spec sif_true //.
+Qed.
+
+Definition riscv_test_regs (x10 x11 : bv 64) : reg_map :=
+    <[ "PC" := RVal_Bits [BV{64} 0x0000000010300000] ]> $
+    <[ "x10" := RVal_Bits x10 ]> $
+    <[ "x11" := RVal_Bits x11 ]> $
+    <[ "misa" := RegVal_Struct [("bits", RVal_Bits misa_bits)] ]> $
+    ∅.
+
+Definition riscv_test_state_global := {|
+    seq_instrs :=
+    <[ [BV{64} 0x0000000010300000] := a0]> $
+    <[ [BV{64} 0x0000000010300004] := a4]> $
+    <[ [BV{64} 0x0000000010300008] := a8]> $
+    ∅;
+    seq_mem := ∅
+|}.
+
+Lemma riscv_test_adequate x10 x11 κs n t2 σ2:
+  nsteps n (initial_local_state <$> [riscv_test_regs x10 x11],
+            riscv_test_state_global) κs (t2, σ2) →
+  (∀ e2, e2 ∈ t2 → not_stuck e2 σ2) ∧ riscv_test_spec x11 κs.
+Proof.
+  set Σ : gFunctors := #[islaΣ].
+  apply: (isla_adequacy Σ) => //.
+  { unfold riscv_test_spec. destruct (decide ((bv_unsigned x11 = 1))); spec_solver. }
+  iIntros (?) "#Hi #Hbm Hspec /= !>". iSplitL => //.
+  iIntros (?).
+  do 4 (rewrite big_sepM_insert; [|by vm_compute]).
+  iIntros "(?&?&?&?&?)".
+  iApply wp_asm_thread_ctx. iIntros (?) "Hctx". iModIntro. iFrame.
+  iApply (wp_next_instr_pre with "[$] []").
+  - iApply (riscv_test x11).
+    all: try by unshelve iApply (instr_intro with "Hi").
+  - repeat liAStep.
+Qed.
