sail-riscv/test.v
@@ -2,7 +2,10 @@ Require Import Sail.Base.
 Require Import Sail.State_monad.
 Require Import Sail.State_lifting.
 Require Import isla.sail_riscv.sail_opsem.
+Require Import isla.automation.
 From isla.instructions.riscv64_test Require Import instrs.
+Require Import isla.examples.riscv64_test.
+
 
 (* Eval hnf in riscv.decode (Ox"00a5b533") >>= execute. *)
 (* Eval vm_compute in decodeCompressed (Ox"8526"). *)
@@ -212,6 +215,7 @@ Ltac red_monad_sim :=
          | |- sim _ _ _ (Smt (DefineConst _ _) _::_)  => apply: sim_DefineConst; [simpl; done|]
          | |- sim _ _ _ (Smt (Assert _) _::_)  => apply: sim_Assert; [simpl; shelve|]
          | |- sim _ _ _ (Branch _ _ _::_)  => apply: sim_Branch
+         | |- sim _ _ _ (BranchAddress _ _::_)  => apply: sim_BranchAddress
          | |- sim _ _ _ (Assume _ _::_)  => let H := fresh "Hassume" in apply: sim_Assume => H; simpl in H
          | |- sim _ (read_reg _) _ (ReadReg _ _ _ _::_)  => apply: sim_read_reg; [done | done | try done; shelve|]
          | |- sim _ (write_reg nextPC_ref _) _ _  => apply: sim_write_reg_private; [done..|]
@@ -221,7 +225,7 @@ Ltac red_monad_sim :=
          end.
 
 Ltac unfold_sim :=
-  unfold wX_bits, rX_bits, rX, wX, regval_from_reg, regval_into_reg, returnm, set.
+  unfold wX_bits, rX_bits, rX, wX, set_next_pc, regval_from_reg, regval_into_reg, returnm, set.
 
 Ltac red_sim :=
     repeat first [
@@ -327,29 +331,88 @@ Proof.
   - simpl. destruct regs => /=. rewrite mword_to_bv_add_vec //.
 Qed.
 
+Lemma getBit_get_word_testbit n2 n z (w : mword n):
+  n = Z.of_N n2 → (0 < n) →
+  getBit (get_word w) z = Z.testbit (bv_unsigned (mword_to_bv (n2:=n2) w)) (Z.of_nat z).
+Proof.
+  move => Heq ?. unfold getBit.
+Admitted.
+
 Lemma sim_instr_a8:
   sim_instr (Uncompressed [BV{32} 0x00b50463]) a8.
 Proof.
   move => regs.
   destruct (eq_vec (x10 regs) (x11 regs)) eqn: Hb1.
-  all: eexists _; split; [by left|].
+  all: eexists _; split. 1: by right; left. 2: by left.
   all: unfold step_cpu; red_sim; unfold execute; red_sim.
   all: unfold execute_BTYPE; red_sim.
   all: apply: sim_read_reg_l; [done|]; red_sim.
-Admitted.
-(*
-
-  rewrite Hb1; red_sim.
-  unfold access_vec_dec, access_mword_dec.
-  match goal with
-  | |- context [getBit ?w ?n] => destruct (getBit w n) eqn:Hbit
-  end.
-  all: red_sim.
-  all: admit.
+  all: rewrite x10_nextPC x11_nextPC Hb1; red_sim.
+  rewrite bit_to_bool_false; [|shelve]. red_sim.
   Unshelve.
-  all: try done.
-  - admit.
-  - admit.
-  - simpl. rewrite mword_to_bv_add_vec //.
+  all: rewrite /= ?x10_nextPC ?x11_nextPC ?PC_nextPC ?nextPC_nextPC; simpl; try done.
+  - rewrite (eq_vec_to_bv 64) // in Hb1. by rewrite Hb1.
+  - move: Hassume. normalize_and_simpl_goal => //= Hb.
+    have Hbit : (Z.testbit (bv_unsigned (mword_to_bv (n2:=64) (PC regs))) 1) = false. { admit. }
+    bitify_hyp Hb. move: (Hb 0 ltac:(done)) => {}Hb.
+    bits_simplify_hyp Hb.
+    rewrite Z.add_bit1 Hbit andb_false_r in Hb. done.
+  - move: Hassume. normalize_and_simpl_goal => //=.
+    have Hbit : (Z.testbit (bv_unsigned (mword_to_bv (n2:=64) (PC regs))) 1) = false. { admit. }
+    bits_simplify. have ? : n = 0 by lia. subst.
+    by rewrite Z.add_bit1 Hbit andb_false_r.
+  - rewrite (eq_vec_to_bv 64) // in Hb1. by rewrite Hb1.
+  - rewrite mword_to_bv_add_vec //.
+  - move: Hassume. normalize_and_simpl_goal => //=.
+    apply bitU_of_bool_B0.
+    rewrite (getBit_get_word_testbit 64) // mword_to_bv_add_vec //=.
+    match goal with
+    | |- context [@mword_to_bv ?n1 ?n2 ?b] => reduce_closed (@mword_to_bv n1 n2 b)
+    end.
+    rewrite bv_add_unsigned bv_wrap_spec_low // Z.add_bit1 /=.
+    repeat match goal with
+    | |- context [Z.testbit ?n1 ?n2] => reduce_closed (Z.testbit n1 n2)
+    end.
+    have -> : (Z.testbit (bv_unsigned (mword_to_bv (n2:=64) (PC regs))) 1) = false. { admit. }
+    by rewrite andb_false_r.
+  - rewrite mword_to_bv_add_vec //.
 Admitted.
-*)
+
+Definition riscv_test_sail_instrs : gmap addr encoded_instruction :=
+  <[ [BV{64} 0x0000000010300000] := Uncompressed [BV{32} 0x00000513]]> $
+  <[ [BV{64} 0x0000000010300004] := Uncompressed [BV{32} 0x00150513]]> $
+  <[ [BV{64} 0x0000000010300008] := Uncompressed [BV{32} 0x00b50463]]> $
+  ∅.
+
+Definition riscv_test_initial_sail_state (regs : regstate) : sail_state :=
+  SAIL (Done tt) regs ∅ riscv_test_sail_instrs false.
+
+Lemma riscv_test_safe regs (x11v : bv 64):
+  PC regs = bv_to_mword [BV{64} 0x0000000010300000] →
+  x11 regs = bv_to_mword x11v →
+  misa regs = {| Misa_Misa_chunk_0 := bv_to_mword misa_bits |} →
+  safe sail_module (riscv_test_initial_sail_state regs) ∧
+    (∀ κs σ', steps sail_module (riscv_test_initial_sail_state regs) κs σ' → riscv_test_spec x11v κs).
+Proof.
+  move => HPC Hx11 Hmisa.
+  apply: iris_transfer_refines.
+  { apply iris_module_wf_isla_lang. }
+  { apply riscv_test_adequate. }
+  apply: sim_implies_refines.
+  - rewrite !dom_insert_L !dom_empty_L. set_solver.
+  - move => ???.
+    repeat move => /lookup_insert_Some[[??]|[? ]]; simplify_map_eq => //.
+    all: unfold get_regval; simpl => ?; simplify_eq.
+    + by rewrite HPC.
+    + done.
+    + rewrite Hx11 /= mword_to_bv_to_mword //.
+    + rewrite Hmisa /= mword_to_bv_to_mword //.
+  - done.
+  - unfold riscv_test_sail_instrs. move => ??? Hsail.
+    repeat move => /lookup_insert_Some[[??]|[? ]]; simplify_map_eq.
+    + apply sim_instr_a0.
+    + apply sim_instr_a4.
+    + apply sim_instr_a8.
+Qed.
+
+(* Print Assumptions riscv_test_safe. *)
