theories/automation.v
@@ -4,9 +4,9 @@ From isla Require Export lifting bitvector_auto.
 Set Default Proof Using "Type".
 
 (* TODO: upstream *)
-(** ** [Done] *)
-Class Done (P : Prop) : Prop := done_proof : P.
-Global Hint Extern 1 (Done ?P) => (change P; done) : typeclass_instances.
+(** ** [TCDone] *)
+Class TCDone (P : Prop) : Prop := done_proof : P.
+Global Hint Extern 1 (TCDone ?P) => (change P; done) : typeclass_instances.
 
 (** * Simplification and normalization hints *)
 Create HintDb isla_coq_rewrite discriminated.
@@ -89,25 +89,25 @@ Global Instance ite_0_1_neq_0_simpl b :
   SimplBoth (ite b [BV{1} 0] [BV{1} 1] ≠ [BV{1} 0]) (b = false).
 Proof. by destruct b. Qed.
 
-Global Instance simpl_bool_to_bv_1 n b1 b2 `{!Done (n ≠ 0%N ∧ bv_unsigned b2 = 1)}:
+Global Instance simpl_bool_to_bv_1 n b1 b2 `{!TCDone (n ≠ 0%N ∧ bv_unsigned b2 = 1)}:
   SimplBothRel (=) (bool_to_bv n b1) b2 (b1 = true).
 Proof.
-  unfold Done in *. split; rewrite bv_eq; rewrite bool_to_bv_unsigned //; destruct b1 => //=; lia.
+  unfold TCDone in *. split; rewrite bv_eq; rewrite bool_to_bv_unsigned //; destruct b1 => //=; lia.
 Qed.
-Global Instance simpl_bool_to_bv_0 n b1 b2 `{!Done (n ≠ 0%N ∧ bv_unsigned b2 = 0)}:
+Global Instance simpl_bool_to_bv_0 n b1 b2 `{!TCDone (n ≠ 0%N ∧ bv_unsigned b2 = 0)}:
   SimplBothRel (=) (bool_to_bv n b1) b2 (b1 = false).
 Proof.
-  unfold Done in *. split; rewrite bv_eq; rewrite bool_to_bv_unsigned //; destruct b1 => //=; lia.
+  unfold TCDone in *. split; rewrite bv_eq; rewrite bool_to_bv_unsigned //; destruct b1 => //=; lia.
 Qed.
-Global Instance simpl_bool_to_bv_neq_1 n b1 b2 `{!Done (n ≠ 0%N ∧ bv_unsigned b2 = 1)}:
+Global Instance simpl_bool_to_bv_neq_1 n b1 b2 `{!TCDone (n ≠ 0%N ∧ bv_unsigned b2 = 1)}:
   SimplBoth (bool_to_bv n b1 ≠ b2) (b1 = false).
 Proof.
-  unfold Done in *. split; rewrite bv_eq; rewrite bool_to_bv_unsigned //; destruct b1 => //=; lia.
+  unfold TCDone in *. split; rewrite bv_eq; rewrite bool_to_bv_unsigned //; destruct b1 => //=; lia.
 Qed.
-Global Instance simpl_bool_to_bv_neq_0  n b1 b2 `{!Done (n ≠ 0%N ∧ bv_unsigned b2 = 0)}:
+Global Instance simpl_bool_to_bv_neq_0  n b1 b2 `{!TCDone (n ≠ 0%N ∧ bv_unsigned b2 = 0)}:
   SimplBoth (bool_to_bv n b1 ≠ b2) (b1 = true).
 Proof.
-  unfold Done in *. split; rewrite bv_eq; rewrite bool_to_bv_unsigned //; destruct b1 => //=; lia.
+  unfold TCDone in *. split; rewrite bv_eq; rewrite bool_to_bv_unsigned //; destruct b1 => //=; lia.
 Qed.
 
 Global Instance simpl_SWriteMem a1 a2 v1 v2:
