sail-riscv/RV64.v
@@ -1,4 +1,3 @@
-Require Import refinedc.lithium.base.
 Require Export Sail.Base.
 Require Export Sail.Prompt_monad.
 Require Export RV64.riscv_types.
@@ -6,11 +5,193 @@ Require Export RV64.mem_metadata.
 Require Export RV64.riscv_extras.
 Require Export RV64.riscv.
 
+Lemma regstate_eta (regs : regstate) :
+  regs = {|
+    satp := satp regs;
+    tlb48 := tlb48 regs;
+    tlb39 := tlb39 regs;
+    htif_payload_writes := htif_payload_writes regs;
+    htif_cmd_write := htif_cmd_write regs;
+    htif_exit_code := htif_exit_code regs;
+    htif_done := htif_done regs;
+    htif_tohost := htif_tohost regs;
+    mtimecmp := mtimecmp regs;
+    fcsr := fcsr regs;
+    f31 := f31 regs;
+    f30 := f30 regs;
+    f29 := f29 regs;
+    f28 := f28 regs;
+    f27 := f27 regs;
+    f26 := f26 regs;
+    f25 := f25 regs;
+    f24 := f24 regs;
+    f23 := f23 regs;
+    f22 := f22 regs;
+    f21 := f21 regs;
+    f20 := f20 regs;
+    f19 := f19 regs;
+    f18 := f18 regs;
+    f17 := f17 regs;
+    f16 := f16 regs;
+    f15 := f15 regs;
+    f14 := f14 regs;
+    f13 := f13 regs;
+    f12 := f12 regs;
+    f11 := f11 regs;
+    f10 := f10 regs;
+    f9 := f9 regs;
+    f8 := f8 regs;
+    f7 := f7 regs;
+    f6 := f6 regs;
+    f5 := f5 regs;
+    f4 := f4 regs;
+    f3 := f3 regs;
+    f2 := f2 regs;
+    f1 := f1 regs;
+    f0 := f0 regs;
+    float_fflags := float_fflags regs;
+    float_result := float_result regs;
+    utval := utval regs;
+    ucause := ucause regs;
+    uepc := uepc regs;
+    uscratch := uscratch regs;
+    utvec := utvec regs;
+    pmpaddr15 := pmpaddr15 regs;
+    pmpaddr14 := pmpaddr14 regs;
+    pmpaddr13 := pmpaddr13 regs;
+    pmpaddr12 := pmpaddr12 regs;
+    pmpaddr11 := pmpaddr11 regs;
+    pmpaddr10 := pmpaddr10 regs;
+    pmpaddr9 := pmpaddr9 regs;
+    pmpaddr8 := pmpaddr8 regs;
+    pmpaddr7 := pmpaddr7 regs;
+    pmpaddr6 := pmpaddr6 regs;
+    pmpaddr5 := pmpaddr5 regs;
+    pmpaddr4 := pmpaddr4 regs;
+    pmpaddr3 := pmpaddr3 regs;
+    pmpaddr2 := pmpaddr2 regs;
+    pmpaddr1 := pmpaddr1 regs;
+    pmpaddr0 := pmpaddr0 regs;
+    pmp15cfg := pmp15cfg regs;
+    pmp14cfg := pmp14cfg regs;
+    pmp13cfg := pmp13cfg regs;
+    pmp12cfg := pmp12cfg regs;
+    pmp11cfg := pmp11cfg regs;
+    pmp10cfg := pmp10cfg regs;
+    pmp9cfg := pmp9cfg regs;
+    pmp8cfg := pmp8cfg regs;
+    pmp7cfg := pmp7cfg regs;
+    pmp6cfg := pmp6cfg regs;
+    pmp5cfg := pmp5cfg regs;
+    pmp4cfg := pmp4cfg regs;
+    pmp3cfg := pmp3cfg regs;
+    pmp2cfg := pmp2cfg regs;
+    pmp1cfg := pmp1cfg regs;
+    pmp0cfg := pmp0cfg regs;
+    tselect := tselect regs;
+    stval := stval regs;
+    scause := scause regs;
+    sepc := sepc regs;
+    sscratch := sscratch regs;
+    stvec := stvec regs;
+    sideleg := sideleg regs;
+    sedeleg := sedeleg regs;
+    mhartid := mhartid regs;
+    marchid := marchid regs;
+    mimpid := mimpid regs;
+    mvendorid := mvendorid regs;
+    minstret_written := minstret_written regs;
+    minstret := minstret regs;
+    mtime := mtime regs;
+    mcycle := mcycle regs;
+    mcountinhibit := mcountinhibit regs;
+    scounteren := scounteren regs;
+    mcounteren := mcounteren regs;
+    mscratch := mscratch regs;
+    mtval := mtval regs;
+    mepc := mepc regs;
+    mcause := mcause regs;
+    mtvec := mtvec regs;
+    medeleg := medeleg regs;
+    mideleg := mideleg regs;
+    mie := mie regs;
+    mip := mip regs;
+    mstatus := mstatus regs;
+    mstatush := mstatush regs;
+    misa := misa regs;
+    cur_inst := cur_inst regs;
+    cur_privilege := cur_privilege regs;
+    x31 := x31 regs;
+    x30 := x30 regs;
+    x29 := x29 regs;
+    x28 := x28 regs;
+    x27 := x27 regs;
+    x26 := x26 regs;
+    x25 := x25 regs;
+    x24 := x24 regs;
+    x23 := x23 regs;
+    x22 := x22 regs;
+    x21 := x21 regs;
+    x20 := x20 regs;
+    x19 := x19 regs;
+    x18 := x18 regs;
+    x17 := x17 regs;
+    x16 := x16 regs;
+    x15 := x15 regs;
+    x14 := x14 regs;
+    x13 := x13 regs;
+    x12 := x12 regs;
+    x11 := x11 regs;
+    x10 := x10 regs;
+    x9 := x9 regs;
+    x8 := x8 regs;
+    x7 := x7 regs;
+    x6 := x6 regs;
+    x5 := x5 regs;
+    x4 := x4 regs;
+    x3 := x3 regs;
+    x2 := x2 regs;
+    x1 := x1 regs;
+    instbits := instbits regs;
+    nextPC := nextPC regs;
+    PC := PC regs;
+  |}.
+Proof. now destruct regs. Qed.
+
+Lemma x10_nextPC regs n:
+  (x10 {[ regs with nextPC := n ]} ) = x10 regs.
+Proof. now rewrite (regstate_eta regs). Qed.
+Lemma x11_nextPC regs n:
+  (x11 {[ regs with nextPC := n ]} ) = x11 regs.
+Proof. now rewrite (regstate_eta regs). Qed.
+Lemma PC_nextPC regs n:
+  (PC {[ regs with nextPC := n ]} ) = PC regs.
+Proof. now rewrite (regstate_eta regs). Qed.
+Lemma nextPC_nextPC regs n:
+  (nextPC {[ regs with nextPC := n ]} ) = n.
+Proof. now rewrite (regstate_eta regs). Qed.
+
+(* This breaks the `with` notations so we have to import it later. *)
+Require Import refinedc.lithium.base.
+
 (* This file should not depend on anything in isla-coq since it is quite slow to compile. *)
 
 Lemma get_word_word_binop {n} f (b1 b2 : mword n):
   get_word (word_binop f b1 b2) = f _ (get_word b1) (get_word b2).
 Proof. by destruct n. Qed.
+
+Lemma get_word_to_word n H (w : Word.word (Z.to_nat n)):
+  get_word (to_word H w) = w.
+Proof. destruct n => //. Qed.
+
+Lemma lt_Npow2 n n1:
+  (0 ≤ n1)%Z →
+  (n < NatLib.Npow2 (Z.to_nat n1))%N ↔ (Z.of_N n < 2 ^ n1)%Z.
+Proof.
+  move => ?.
+  rewrite -Npow2_pow Z_nat_N. etrans; [ apply N2Z.inj_lt |].
+  by rewrite N2Z.inj_pow Z2N.id.
+Qed.
 
 Lemma get_set_regval r regs regs' v:
   set_regval r v regs = Some regs' ->
@@ -54,3 +235,20 @@ Proof.
   Unshelve.
   (* all: clear Hcase; move => ?; subst r; simpl; move: Hset; repeat (apply Hcase2; [shelve|]); done. *)
 Admitted.
+
+Lemma bit_to_bool_false b:
+  b = B0 →
+  bit_to_bool b = Done false.
+Proof. by move => ->. Qed.
+Lemma bit_to_bool_true b:
+  b = B1 →
+  bit_to_bool b = Done true.
+Proof. by move => ->. Qed.
+Lemma bitU_of_bool_B0 b :
+  b = false →
+  bitU_of_bool b = B0.
+Proof. by move => ->. Qed.
+Lemma bitU_of_bool_B1 b :
+  b = true →
+  bitU_of_bool b = B1.
+Proof. by move => ->. Qed.
